src/ContainersOps.dfy
@@ -5,17 +5,17 @@ include "Ord.dfy"
  *  [startIdx, endIdx) of the input sequence a.
  */
 ghost function mapSeq<T,R>(a: seq<T>, f: T -> R, startIdx: nat, endIdx: nat): (output: seq<R>)
-	requires 0 <= startIdx <= endIdx <= |a|
-	ensures |output| == endIdx-startIdx
-	ensures forall i: nat | 0 <= i < |output| :: output[i] == f(a[startIdx + i])
-	decreases endIdx - startIdx
+  requires 0 <= startIdx <= endIdx <= |a|
+  ensures |output| == endIdx-startIdx
+  ensures forall i: nat | 0 <= i < |output| :: output[i] == f(a[startIdx + i])
+  decreases endIdx - startIdx
 {
-  if(startIdx == endIdx) then []
+  if (startIdx == endIdx) then []
   else [f(a[startIdx])] + mapSeq(a, f, startIdx + 1, endIdx)
 }
 
 lemma mapSeqConcatChg<T,R>(a: seq<T>, b: seq<T>, f: T->R) // Generalize to startIdx, endIdx?
-	ensures mapSeq(a+b, f, 0, |a+b|) == mapSeq(a, f, 0, |a|) + mapSeq(b, f, 0, |b|)
+  ensures mapSeq(a+b, f, 0, |a+b|) == mapSeq(a, f, 0, |a|) + mapSeq(b, f, 0, |b|)
 {}
 
 /*
@@ -23,30 +23,30 @@ lemma mapSeqConcatChg<T,R>(a: seq<T>, b: seq<T>, f: T->R) // Generalize to start
  * "b" sequence
  */
 ghost function selectSeq<T>(a: seq<T>, b: seq<bool>, startIdx: nat, endIdx: nat): (output: seq<T>)
-	requires 0 <= startIdx <= endIdx <= |a|// == |b|
-	requires endIdx <= |b|
-	ensures |output| <= (endIdx-startIdx) <= |a|
-	ensures forall i: nat | 0 <= i < |output| :: output[i] in a
-	ensures forall i: nat | startIdx <= i < endIdx :: b[i] == true ==> a[i] in output
-	decreases endIdx - startIdx
+  requires 0 <= startIdx <= endIdx <= |a|// == |b|
+  requires endIdx <= |b|
+  ensures |output| <= (endIdx-startIdx) <= |a|
+  ensures forall i: nat | 0 <= i < |output| :: output[i] in a
+  ensures forall i: nat | startIdx <= i < endIdx :: b[i] == true ==> a[i] in output
+  decreases endIdx - startIdx
 {
   if(startIdx == endIdx) then []
   else (if(b[startIdx]) then [a[startIdx]] else []) + selectSeq(a, b, startIdx + 1, endIdx)
 }
 
 lemma selectSeqZero<T>(a: seq<T>, b: seq<bool>, startIdx: nat, endIdx: nat)
-	requires 0 <= startIdx <= endIdx <= |a|// == |b|
-	requires endIdx <= |b|
-	requires forall i: nat | startIdx <= i < endIdx :: b[i] == false
-	ensures selectSeq(a, b, startIdx, endIdx) == []
-	decreases endIdx - startIdx
+  requires 0 <= startIdx <= endIdx <= |a|// == |b|
+  requires endIdx <= |b|
+  requires forall i: nat | startIdx <= i < endIdx :: b[i] == false
+  ensures selectSeq(a, b, startIdx, endIdx) == []
+  decreases endIdx - startIdx
 {
-	if(startIdx == endIdx) {
-		assert selectSeq(a, b, startIdx, endIdx) == [];
-	} else {
-		selectSeqZero(a, b, startIdx+1, endIdx);
-		assert b[startIdx] == false;
-	}
+  if(startIdx == endIdx) {
+    assert selectSeq(a, b, startIdx, endIdx) == [];
+  } else {
+    selectSeqZero(a, b, startIdx+1, endIdx);
+    assert b[startIdx] == false;
+  }
 }
 
 
@@ -55,23 +55,23 @@ lemma selectSeqZero<T>(a: seq<T>, b: seq<bool>, startIdx: nat, endIdx: nat)
  * with each sequence is the same
  */
 lemma selectSeqEqualB<T>(a: seq<T>, b1: seq<bool>, b2: seq<bool>, startIdx: nat, endIdx: nat)
-	requires 0 <= startIdx <= endIdx <= |a|// == |b1| == |b2|
-	requires endIdx <= |b1|
-	requires endIdx <= |b2|
-	requires forall i: nat | startIdx <= i < endIdx :: b1[i] == b2[i]
-	ensures  selectSeq(a, b1, startIdx, endIdx) == selectSeq(a, b2, startIdx, endIdx)
-	decreases endIdx - startIdx
+  requires 0 <= startIdx <= endIdx <= |a|// == |b1| == |b2|
+  requires endIdx <= |b1|
+  requires endIdx <= |b2|
+  requires forall i: nat | startIdx <= i < endIdx :: b1[i] == b2[i]
+  ensures  selectSeq(a, b1, startIdx, endIdx) == selectSeq(a, b2, startIdx, endIdx)
+  decreases endIdx - startIdx
 {
-	if(startIdx == endIdx) {
-		calc == {
-			selectSeq(a, b1, startIdx, endIdx);
-			[];
-			selectSeq(a, b2, startIdx, endIdx);
-		}
-	} else {
-		selectSeqEqualB(a, b1, b2, startIdx+1, endIdx);
-		assert selectSeq(a, b1, startIdx+1, endIdx) == selectSeq(a, b2, startIdx+1, endIdx);
-	}
+  if(startIdx == endIdx) {
+    calc == {
+      selectSeq(a, b1, startIdx, endIdx);
+      [];
+      selectSeq(a, b2, startIdx, endIdx);
+    }
+  } else {
+    selectSeqEqualB(a, b1, b2, startIdx+1, endIdx);
+    assert selectSeq(a, b1, startIdx+1, endIdx) == selectSeq(a, b2, startIdx+1, endIdx);
+  }
 }
 
 
@@ -80,39 +80,39 @@ lemma selectSeqEqualB<T>(a: seq<T>, b1: seq<bool>, b2: seq<bool>, startIdx: nat,
  * is added to the output
  */
 lemma selectSeqDif<T>(a: seq<T>, b: seq<bool>, difIdx: nat, startIdx: nat, endIdx: nat)
-	requires 0 <= startIdx <= difIdx < endIdx <= |a| == |b|
-	requires b[difIdx] == false
-	ensures selectSeq(a, b[difIdx := true], startIdx, endIdx) == selectSeq(a, b, startIdx, difIdx) + [a[difIdx]] + selectSeq(a, b, difIdx+1, endIdx)
-	decreases endIdx - startIdx
+  requires 0 <= startIdx <= difIdx < endIdx <= |a| == |b|
+  requires b[difIdx] == false
+  ensures selectSeq(a, b[difIdx := true], startIdx, endIdx) == selectSeq(a, b, startIdx, difIdx) + [a[difIdx]] + selectSeq(a, b, difIdx+1, endIdx)
+  decreases endIdx - startIdx
 {
-	if(startIdx == endIdx-1) {
-		assert difIdx == startIdx;
-		calc == {
-			selectSeq(a, b[difIdx := true], startIdx, endIdx);
-			[a[difIdx]] + selectSeq(a, b, startIdx+1, endIdx); {assert b[difIdx] == false;}
-			[a[difIdx]] + selectSeq(a, b, startIdx, endIdx);
-		}
-	} else if(difIdx == startIdx){
-		assert selectSeq(a, b[startIdx := true], startIdx, endIdx) == [a[difIdx]] + selectSeq(a, b[startIdx := true], startIdx+1, endIdx);
-		selectSeqEqualB(a, b, b[startIdx := true], startIdx+1, endIdx);
-	} else {
-		selectSeqDif(a, b, difIdx, startIdx + 1, endIdx);
-	}
+  if(startIdx == endIdx-1) {
+    assert difIdx == startIdx;
+    calc == {
+      selectSeq(a, b[difIdx := true], startIdx, endIdx);
+      [a[difIdx]] + selectSeq(a, b, startIdx+1, endIdx); {assert b[difIdx] == false;}
+      [a[difIdx]] + selectSeq(a, b, startIdx, endIdx);
+    }
+  } else if(difIdx == startIdx){
+    assert selectSeq(a, b[startIdx := true], startIdx, endIdx) == [a[difIdx]] + selectSeq(a, b[startIdx := true], startIdx+1, endIdx);
+    selectSeqEqualB(a, b, b[startIdx := true], startIdx+1, endIdx);
+  } else {
+    selectSeqDif(a, b, difIdx, startIdx + 1, endIdx);
+  }
 }
 
 lemma selectSeqSplit<T>(a: seq<T>, b: seq<bool>, splitIdx: nat, startIdx: nat, endIdx: nat)
-	decreases endIdx-startIdx
-	requires startIdx <= splitIdx < endIdx <= |a|
-	requires endIdx <= |b|
-	ensures selectSeq(a, b, startIdx, endIdx) == selectSeq(a, b, startIdx, splitIdx) + selectSeq(a, b, splitIdx, endIdx)
+  decreases endIdx-startIdx
+  requires startIdx <= splitIdx < endIdx <= |a|
+  requires endIdx <= |b|
+  ensures selectSeq(a, b, startIdx, endIdx) == selectSeq(a, b, startIdx, splitIdx) + selectSeq(a, b, splitIdx, endIdx)
 {
-	if(startIdx == splitIdx) {
-		assert selectSeq(a, b, startIdx, splitIdx) == [];
-		assert selectSeq(a, b, startIdx, endIdx) == selectSeq(a, b, splitIdx, endIdx);
-		assert selectSeq(a, b, startIdx, endIdx) == selectSeq(a, b, startIdx, splitIdx) + selectSeq(a, b, splitIdx, endIdx);
-	} else {
-		selectSeqSplit(a, b, splitIdx, startIdx+1, endIdx);
-	}
+  if(startIdx == splitIdx) {
+    assert selectSeq(a, b, startIdx, splitIdx) == [];
+    assert selectSeq(a, b, startIdx, endIdx) == selectSeq(a, b, splitIdx, endIdx);
+    assert selectSeq(a, b, startIdx, endIdx) == selectSeq(a, b, startIdx, splitIdx) + selectSeq(a, b, splitIdx, endIdx);
+  } else {
+    selectSeqSplit(a, b, splitIdx, startIdx+1, endIdx);
+  }
 }
 
 /*
@@ -120,32 +120,32 @@ lemma selectSeqSplit<T>(a: seq<T>, b: seq<bool>, splitIdx: nat, startIdx: nat, e
  * is not added to the output
  */
 lemma selectSeqDecompose<T>(a: seq<T>, b: seq<bool>, difIdx: nat, startIdx: nat, endIdx: nat)
-	requires 0 <= startIdx <= difIdx < endIdx <= |a|// == |b|
-	requires endIdx <= |b|
-	requires b[difIdx] == false
-	ensures selectSeq(a, b, startIdx, endIdx) == selectSeq(a, b, startIdx, difIdx) + selectSeq(a, b, difIdx+1, endIdx)
-	decreases endIdx - startIdx
+  requires 0 <= startIdx <= difIdx < endIdx <= |a|// == |b|
+  requires endIdx <= |b|
+  requires b[difIdx] == false
+  ensures selectSeq(a, b, startIdx, endIdx) == selectSeq(a, b, startIdx, difIdx) + selectSeq(a, b, difIdx+1, endIdx)
+  decreases endIdx - startIdx
 {
-	if(startIdx == endIdx-1) {
-		assert difIdx == startIdx;
-		calc == {
-			selectSeq(a, b[difIdx := false], startIdx, endIdx);
-			selectSeq(a, b, startIdx+1, endIdx); {assert b[difIdx] == false;}
-			selectSeq(a, b, startIdx+1, endIdx);
-		}
-	} else if(difIdx == startIdx){
-		assert selectSeq(a, b[startIdx := false], startIdx, endIdx) == selectSeq(a, b[startIdx := false], startIdx+1, endIdx);
-		selectSeqEqualB(a, b, b[startIdx := false], startIdx+1, endIdx);
-	} else {
-		selectSeqDecompose(a, b, difIdx, startIdx + 1, endIdx);
-	}
+  if(startIdx == endIdx-1) {
+    assert difIdx == startIdx;
+    calc == {
+      selectSeq(a, b[difIdx := false], startIdx, endIdx);
+      selectSeq(a, b, startIdx+1, endIdx); {assert b[difIdx] == false;}
+      selectSeq(a, b, startIdx+1, endIdx);
+    }
+  } else if(difIdx == startIdx){
+    assert selectSeq(a, b[startIdx := false], startIdx, endIdx) == selectSeq(a, b[startIdx := false], startIdx+1, endIdx);
+    selectSeqEqualB(a, b, b[startIdx := false], startIdx+1, endIdx);
+  } else {
+    selectSeqDecompose(a, b, difIdx, startIdx + 1, endIdx);
+  }
 }
 
 ghost function filterSeq<T>(a:seq<T>, b: T -> bool, startIdx: nat, endIdx: nat): (output: seq<T>)
-	requires 0 <= startIdx <= endIdx <= |a|
-	ensures |output| <= (endIdx-startIdx) <= |a|
-	ensures forall i: nat | 0 <= i < |output| :: output[i] in a && b(output[i]) == true
-	decreases endIdx - startIdx
+  requires 0 <= startIdx <= endIdx <= |a|
+  ensures |output| <= (endIdx-startIdx) <= |a|
+  ensures forall i: nat | 0 <= i < |output| :: output[i] in a && b(output[i]) == true
+  decreases endIdx - startIdx
 {
   if(startIdx == endIdx) then []
   else ((if(b(a[startIdx])) then [a[startIdx]] else []) + filterSeq(a, b, startIdx + 1, endIdx))
