src/Especificacion.dfy
@@ -1,0 +1,16 @@
+//A nivel de especificación tenemos estos datatype
+
+datatype ItemData = ItemData(weight: real, value: real) {
+  ghost predicate Valid() {
+    weight > 0.0 && value > 0.0
+  }
+}
+
+datatype SolutionData = SolutionData(itemsAssign: seq<bool>, totalWeight: real, totalValue: real, k: int) {
+  ghost function Valid(itemsD: seq<ItemData>, maxWeight: real) : bool {
+    0 <= k <= |itemsAssign| &&
+    |itemsAssign| == |itemsD|
+    && totalWeight <= maxWeight    
+  }
+
+}
