src/InputData.dfy
@@ -1,9 +1,0 @@
-class InputData {
-    var weight: real
-    var value: real
-
-    constructor(w: real, v: real) {
-        this.weight := w;
-        this.value := v;
-    }
-}
