src/Item.dfy
@@ -1,0 +1,16 @@
+class Item {
+  const weight: real
+  const value:  real
+
+  constructor(w: real, v: real) {
+    this.weight := w;
+    this.value := v;
+  }
+
+  ghost predicate Valid () {
+    this.weight > 0.0 && this.value > 0.0
+  }
+
+
+
+}
